
Given the following input:
\begin{table}[ht!]
\begin{center}
\begin{tabular}{|l|r|}
\hline
time & $\mathit{x}1$\\
\hline
1 & $\mathit{cell}_3_2$ \\
2 & $\mathit{cell}_3_1$ \\
3 & $\mathit{cell}_3_2$ \\
4 & $\mathit{cell}_2_2$ \\
5 & $\mathit{cell}_3_2$ \\
6 & $\mathit{cell}_4_2$ \\
7 & $\mathit{cell}_3_2$ \\
8 & $\mathit{cell}_3_3$ \\
9 & $\mathit{cell}_3_2$ \\
\hline
\end{tabular}
\end{center}
\end{table}

Our system produces the frame $\phi = (T, O, P, V)$, where:
\begin{equation*}
\phi = \left \{
\begin{aligned}
& T = \{ 
1,cell
\}\\
& O = \{
\mathit{cell}_1_1: cell,\mathit{cell}_1_2: cell,\mathit{cell}_1_3: cell,\mathit{cell}_2_1: cell,\mathit{cell}_2_2: cell,\mathit{cell}_2_3: cell,\mathit{cell}_3_1: cell,\mathit{cell}_3_2: cell,\mathit{cell}_3_3: cell,\mathit{cell}_4_1: cell,\mathit{cell}_4_2: cell,\mathit{cell}_4_3: cell,\mathit{cell}_5_1: cell,\mathit{cell}_5_2: cell,\mathit{cell}_5_3: cell,\mathit{x}1: 1
\}\\
& P = \{
\mathit{east}(1),\mathit{in}_1(1, cell),\mathit{noop}(1),\mathit{north}(1),\mathit{south}(1),\mathit{west}(1)
\}\\
& V = \{
1_1: 1,CELL_1: cell,CELL_2: cell
\}\\
\end{aligned}\right\}
\end{equation*}
Our system finds the theory $\theta = (\phi, I, R, C)$, where:
\begin{eqnarray*}
I & = & \left\{ \begin{array}{l}
\mathit{in}_1(\mathit{x}1,\mathit{cell}_3_2)\\
\end{array}\right\}\\
R & = &  \left\{ \begin{array}{l}
\mathit{below}(\mathit{CELL}_1,\mathit{CELL}_2) \wedge \mathit{north}(\mathit{}1_1) \wedge \mathit{in}_1(\mathit{}1_1,\mathit{CELL}_2) \ni \mathit{in}_1(\mathit{}1_1,\mathit{CELL}_1)\\
\mathit{right}(\mathit{CELL}_1,\mathit{CELL}_2) \wedge \mathit{east}(\mathit{}1_1) \wedge \mathit{in}_1(\mathit{}1_1,\mathit{CELL}_1) \ni \mathit{in}_1(\mathit{}1_1,\mathit{CELL}_2)\\
\mathit{below}(\mathit{CELL}_1,\mathit{CELL}_2) \wedge \mathit{south}(\mathit{}1_1) \wedge \mathit{in}_1(\mathit{}1_1,\mathit{CELL}_1) \ni \mathit{in}_1(\mathit{}1_1,\mathit{CELL}_2)\\
\mathit{noop}(\mathit{}1_1) \ni \mathit{west}(\mathit{}1_1)\\
\mathit{right}(\mathit{CELL}_2,\mathit{CELL}_1) \wedge \mathit{west}(\mathit{}1_1) \wedge \mathit{in}_1(\mathit{}1_1,\mathit{CELL}_1) \ni \mathit{in}_1(\mathit{}1_1,\mathit{CELL}_2)\\
\end{array}\right\}\\
C & = & \left\{ \begin{array}{l}
\forall X : 1, \; \exists ! Y : cell, \; in_1(X, Y) \\
\end{array}\right\}\\
\end{eqnarray*}

